incr/ClientIA.v
@@ -1,9 +1,10 @@
 Require Import CRIS.
-Require Import IncrI IncrA SchA MemA SchTactics FAA_A.
+From CRIS.incr Require Import Header ClientI ClientA FaaA.
+Require Import SchA MemA SchTactics.
 From iris Require Import frac_auth numbers.
-
-Module IncrIA. Section IncrIA.
-  Import IncrAS.
+(* Erase *) Require Import ltac2_lib.
+Module ClientIA. Section ClientIA.
+  Import ClientA.
   Context `{_sinvG: !sinvG Γ Σ α β τ _I _S}.
   Context `{_memG: !memG}.
   Context `{_schG: !schG}.
@@ -11,63 +12,63 @@ Module IncrIA. Section IncrIA.
 
   Definition Ist : nat → alist key Any.t → alist key Any.t → iProp Σ := λ _ _ _, emp%I.
 
-  Context (u_s: univ_id).
-  Context `{UGT: u_s > u_t}.
+  Context (E : coPset) (Hsub : ↑N_main ⊆ E).
   Context (sp_s sp_t sp_user_s sp_user_t sp_mem : string → option fspec).
-  Context (SchInSpS : sp_incl (SchAS.sp u_s sp_user_s) sp_s).
-  Context (SchInSpT : sp_incl (SchAS.sp u_t sp_user_t) sp_t).
-  Context (MemInSp : sp_incl MemA.sp sp_s).
-  Context (MainInSp : sp_incl (IncrAS.sp u_s) sp_user_s).
+  Context (SchInSpS : sp_incl (SchAS.sp E sp_user_s) sp_s).
+  (* Context (SchInSpT : sp_incl (SchAS.sp ∅ sp_user_t) sp_t). *)
+  (* Context (MemInSp : sp_incl MemA.sp sp_s). *)
+  Context (MainInSp : sp_incl (ClientA.sp E) sp_user_s).
 
   Local Definition MemA := (MemA.t sp_mem).
-  Local Definition IncrA := (IncrA.t u_s sp_s).
-  Local Definition IncrI := (IncrI.t).
-  Local Definition IstFull := (IstProd (IstSB IncrA.(HMod.scopes) Ist) IstEq).
-  Local Definition MA := (IncrA ★ MemA).
-  Local Definition MI := ((IncrI ★ FaaA.t u_t sp_t) ★ MemA).
+  Local Definition ClientA := (ClientA.t E sp_s).
+  Local Definition ClientI := (ClientI.t).
+  Local Definition IstFull := (IstProd (IstSB ClientA.(HMod.scopes) Ist) IstEq).
+  Local Definition MA := (ClientA ★ MemA).
+  Local Definition MI := ((ClientI ★ FaaA.t) ★ MemA).
 
   Lemma f_spawnable γ v bofs :
-    SchAS.fspec_spawnable u_s (IncrAS.incr_spec u_s)
+    SchAS.fspec_spawnable E (incr_spec E)
       (λ varg arg,
         ⌜varg = arg ∧ varg = ([Vptr bofs]↑↑)⌝
         ∗ counter γ (1/2) v
-        ∗ incr_inv u_s 0 γ bofs)%I
+        ∗ incr_inv 0 γ bofs)%I
       (λ vret ret,
         existT 0 ((⌜vret = ret ∧ vret = tt↑↑⌝ ∗ counter_syn γ (1/2) (v + 2))%SAT)).
   Proof.
-    rewrite /SchAS.fspec_spawnable /wsim_fspec /fspec_virtual /precond /postcond /incr_spec /=.
+    rewrite /SchAS.fspec_spawnable /fspec_sch /fspec_virtual /precond /postcond /incr_spec /=.
     ii; ss. eexists (x0, (bofs, v, γ)); split; red; ii.
-    - rewrite /precond /sch_fspec /fspec_simple /wsim_fspec /precond /=.
+    - rewrite /precond /fspec_sch /fspec_simple /fspec_sch /precond /=.
       iIntros "[W [% [-> [TID [% [-> [[-> ->] [C #INV]]]]]]]]". iFrame. eauto.
-    - rewrite /postcond /sch_fspec /fspec_simple /wsim_fspec /postcond /=.
+    - rewrite /postcond /fspec_sch /fspec_simple /fspec_sch /postcond /=.
       iIntros "[W [TID [[-> C] ->]]]". iFrame. iExists _; iSplitR; eauto.
       iExists _; iSplitR; eauto. SL_red. iSplitR; eauto.
   Qed.
 
   Lemma incr_simF : HSim.sim_fun open MA MI IstFull IncrHdr.incr.
-  Proof using UGT SchInSpS SchInSpT MemInSp MainInSp.
-    init_simF u_s u_t.
+  Proof using SchInSpS MainInSp Hsub.
+    init_simF.
 
     steps_l. iDestruct "ASM" as "[TID [[-> [C #INV]] ->]]". hss.
     destruct q5 as [b ofs]. rename q1 into tid, q4 into γ, q6 into v.
 
     steps_l. hss. steps_l.
     steps_r. hss. steps_r.
-    rewrite /IncrI.incr /IncrA.incr /=. steps_r.
+    rewrite /ClientI.incr /ClientA.incr /=. steps_r.
 
     sch_yield_r.
     iSplitL "IST"; iFrame.
     clear nths NODS NODD. iIntros (nths st_s st_t NODS NODD) "IST TID".
 
     (* tgt inline - faa *)
-    inline_r. hss. steps_r. force_r (tid, (b, ofs)). forces_r. iFrame. iSplit; eauto. steps_r. hss.
-    steps_r.
-
-    sch_yield_r.
+    inline_r. hss. steps_r. force_r (tid, (b, ofs)). forces_r. iFrame. iSplit; eauto.
+    steps_r. hss.
+    steps_r. sch_yield_r.
+    { rewrite /SchAS.sp; unseal CRIS. split; first prove_nodup. refl. }
+    { try set_solver. }
     iSplitL "IST"; iFrame.
     clear nths st_s st_t NODS NODD. iIntros (nths st_s st_t NODS NODD) "IST".
 
-    rewrite /IncrAS.incr_inv.
+    rewrite /incr_inv.
     iInv "INV" as "I" "IA". SL_red.
     iDestruct "I" as (x) "PT". SL_red. iDestruct "PT" as "[PT CA]".
 
@@ -78,10 +79,13 @@ Module IncrIA. Section IncrIA.
     iMod ("IA" with "[GRT CA]") as "_".
     { iExists (x + 1)%Z; SL_red; ss; iFrame. }
 
-    sch_yield_r. iFrame.
+    sch_yield_r.
+    { rewrite /SchAS.sp; unseal CRIS. split; first prove_nodup. refl. }
+    { try set_solver. }
+    iFrame.
     clear nths st_s st_t NODS NODD. iIntros (nths st_s st_t NODS NODD) "IST".
 
-    rewrite /IncrAS.incr_inv.
+    rewrite /incr_inv.
     iInv "INV" as "I" "IA". SL_red.
     clear x. iDestruct "I" as (x) "PT". SL_red. iDestruct "PT" as "[PT CA]".
 
@@ -92,10 +96,12 @@ Module IncrIA. Section IncrIA.
     iMod ("IA" with "[GRT CA]") as "_".
     { iExists (x + 1)%Z; SL_red; ss; iFrame. }
 
-    sch_yield_r. iFrame.
+    sch_yield_r.
+    { rewrite /SchAS.sp; unseal CRIS. split; first prove_nodup. refl. }
+    { try set_solver. }
+    iFrame.
     clear nths st_s st_t NODS NODD. iIntros (nths st_s st_t NODS NODD) "IST".
     steps_r. iDestruct "GRT" as "[TID [-> _]]". hss. steps_r.
-
     sch_yield_r. iFrame.
     clear nths st_s st_t NODS NODD. iIntros (nths st_s st_t NODS NODD) "IST TID".
 
@@ -108,8 +114,8 @@ Module IncrIA. Section IncrIA.
   (*SLOW*)Qed.
 
   Lemma main_simF : HSim.sim_fun open MA MI IstFull IncrHdr.main.
-  Proof using UGT SchInSpS SchInSpT MemInSp MainInSp.
-    init_simF u_s u_t.
+  Proof using SchInSpS MainInSp Hsub.
+    init_simF.
 
     steps_l. iDestruct "ASM" as "[TID [-> ->]]". hss.
     steps_l.
@@ -122,11 +128,9 @@ Module IncrIA. Section IncrIA.
     sch_yield_l.
 
     (* src/tgt alloc *)
-    steps_l. force_l 1. steps_l. force_l. steps_l.
-    force_l. iSplit; eauto. steps_l.
-    steps_r. call "IST".
-    steps_l. iDestruct "ASM" as "[[%b [-> [PT _]]] ->]". hss.
-    steps_r. hss. steps_r.
+    steps_r. inline_r. force_r 1. forces_r. iSplit; first ss. steps_r.
+    iDestruct "GRT" as "[[%blk [-> [PT _]]] ->]". hss_r. steps_r.
+    steps_l. force_l (Vptr (blk, 0%Z)). steps_l.
 
     (* tgt yield *)
     sch_yield_r. iFrame.
@@ -136,7 +140,7 @@ Module IncrIA. Section IncrIA.
     clear nths st_s st_t NODS NODD. iIntros (nths st_s st_t NODS NODD) "IST TID".
 
     (* tgt store *)
-    inline_r. steps_r. force_r (b, 0%Z, _, Vint 0%Z). steps_r.
+    inline_r. steps_r. force_r (blk, 0%Z, _, Vint 0%Z). steps_r.
     force_r. steps_r. force_r. iSplitL "PT".
     { iFrame. eauto. }
     steps_r. iDestruct "GRT" as "[[PT ->] ->]". hss. steps_r.
@@ -145,12 +149,11 @@ Module IncrIA. Section IncrIA.
     sch_yield_r. iFrame.
     clear nths st_s st_t NODS NODD. iIntros (nths st_s st_t NODS NODD) "IST TID".
     sch_yield_l.
-
-    iApply (wsim_own_alloc (●F 0%Z ⋅ ◯F{1} 0%Z)).
+    iApply (wsim_own_alloc ((●F 0%Z ⋅ ◯F{1} 0%Z))).
     { apply frac_auth_valid; ss. }
 
     iIntros "[%γc [A F]]".
-    iMod (inv_alloc (ccounter_syn 0 γc (b, 0%Z)) _ _ _ N_main with "[PT A]") as "#I"; eauto.
+    iMod (inv_alloc (ccounter_syn 0 γc (blk, 0%Z)) _ _ _ N_main with "[PT A]") as "#I"; eauto.
     { rewrite /ccounter_syn; SL_red; iExists 0; SL_red; iFrame. }
     iPoseProof (counter_op with "[F]") as "[F1 F2]".
     { rewrite -Qp.half_half -{2}(Z.add_0_r 0%Z). iApply "F". }
@@ -202,7 +205,7 @@ Module IncrIA. Section IncrIA.
     iCombine "C Q Q2" as "C" gives %[_ WF%frac_auth_agree]. inv WF; ss.
     iDestruct "C" as "[CA CF]".
 
-    inline_r. steps_r. force_r (b, 0%Z, 1%Qp, (Vint 4)). steps_r. forces_r.
+    inline_r. steps_r. force_r (blk, 0%Z, 1%Qp, (Vint 4)). steps_r. forces_r.
     iSplitL "PT"; eauto.
     steps_r. iDestruct "GRT" as "[[PT ->] ->]". hss. steps_r.
 
@@ -234,7 +237,7 @@ Module IncrIA. Section IncrIA.
     { eapply incr_simF. }
     { eapply main_simF. }
   Qed.
-End IncrIA.
+End ClientIA.
 
 Section ctxr.
   Context `{_sinvG: !sinvG Γ Σ α β τ _I _S}.
@@ -242,19 +245,17 @@ Section ctxr.
   Context `{_schG: !schG}.
   Context `{_incrG: !incrG}.
 
-  Definition ctxr (u_s u_t : univ_id) (sp_s sp_t sp_user_s sp_user_t sp_mem : string → option fspec)
-      (SchInSpS : sp_incl (SchAS.sp u_s sp_user_s) sp_s)
-      (SchInSpT : sp_incl (SchAS.sp u_t sp_user_t) sp_t)
-      (MainInSp : sp_incl (IncrAS.sp u_s) sp_user_s)
-      (MemInSp : sp_incl MemA.sp sp_s)
-      (Univ : u_s > u_t) :
+  Definition ctxr (E : coPset) (sp_s sp_user_s sp_mem : string → option fspec) :
+    ↑ClientA.N_main ⊆ E →
+    sp_incl (ClientA.sp E) sp_user_s →
+    sp_incl (SchAS.sp E sp_user_s) sp_s →
     ctx_refines
-      (IncrA.t u_s sp_s          ★ (MemA.t sp_mem), emp%I)
-      (IncrI.t ★ FaaA.t u_t sp_t ★ (MemA.t sp_mem), emp%I).
+      (ClientA.t E sp_s   ★ (MemA.t sp_mem), emp%I)
+      (ClientI.t ★ FaaA.t ★ (MemA.t sp_mem), emp%I).
   Proof.
     etrans; cycle 1. { do 2 ctxr_rotate. ctxr_refl. }
-    eset (GRP := IncrI.t ★ _).
+    eset (GRP := ClientI.t ★ _).
     etrans; cycle 1. { ctxr_rotate. ctxr_refl. }
     eapply main_adequacy, sim; try solve_sch_sp; eauto.
   Qed.
-End ctxr. End IncrIA.
+End ctxr. End ClientIA.
