incr/FaaA.v
@@ -1,16 +1,17 @@
 Require Import CRIS.
-Require Import ImpPrelude IncrHeader MemHeader MemA SchA SchTactics SchHeader.
+Require Import ImpPrelude MemHeader MemA SchA SchTactics SchHeader.
+From CRIS.incr Require Import Header.
 
 Module FaaA. Section FaaA.
   Context `{_sinvG: !sinvG Γ Σ α β τ _I _S}.
   Context `{_memG: !memG}.
   Context `{_schG: !schG}.
 
-  Definition faa2_spec u : fspec :=
-    sch_fspec u (fspec_simple (λ bofs, (λ arg, ⌜arg = [Vptr bofs]↑⌝, λ ret, ⌜ret = tt↑⌝)))%I.
+  Definition faa2_spec : fspec :=
+    fspec_sch ∅ (fspec_simple (λ bofs, (λ arg, ⌜arg = [Vptr bofs]↑⌝, λ ret, ⌜ret = tt↑⌝)))%I.
 
-  Definition sp u : alist string fspec :=
-    [(FaaHdr.faa2, faa2_spec u)].
+  Definition sp : alist string fspec :=
+    [(FaaHdr.faa2, faa2_spec)].
 
   Definition scopes : list string := [].
 
@@ -27,15 +28,15 @@ Module FaaA. Section FaaA.
         trigger (Guarantee ((b, ofs) ↦ Vint (v + 1)));;;
       𝒴;;; Ret tt.
 
-  Definition fnsems u := [(FaaHdr.faa2, (wmask_all, scopes, mk_specbody (faa2_spec u) (cfunN faa2)))].
+  Definition fnsems := [(FaaHdr.faa2, (wmask_all, scopes, mk_specbody faa2_spec (cfunN faa2)))].
 
-  Program Definition Mod u : SMod.t := {|
+  Program Definition Mod : SMod.t := {|
     SMod.scopes := scopes;
-    SMod.fnsems := fnsems u;
+    SMod.fnsems := fnsems;
     SMod.initial_st := [];
   |}.
   Solve All Obligations with prove_scope.
   Next Obligation. prove_nodup. Qed.
 
-  Definition t u sp : HMod.t := Seal.sealing CRIS (SMod.to_hmod sp (Mod u)).
+  Definition t : HMod.t := Seal.sealing CRIS (SMod.to_hmod (to_sp (SchAS.sp ∅ sp_empty)) Mod).
 End FaaA. End FaaA.
