incr/FaaIA.v
@@ -1,34 +1,40 @@
 Require Import CRIS.
-Require Import ImpPrelude IncrHeader MemHeader MemA SchA SchTactics SchHeader.
-Require Import FAA_I FAA_A.
+From CRIS.incr Require Import Header.
+Require Import ImpPrelude MemHeader MemA SchA SchTactics SchHeader.
+Require Import FaaI FaaA.
 
 Module FaaIA. Section FaaIA.
   Context `{_sinvG: !sinvG Γ Σ α β τ _I _S}.
   Context `{_memG: !memG}.
   Context `{_schG: !schG}.
-                
-  Context (u_s : univ_id).
-  Context (sp_s sp_mem sp_user_s : string → option fspec).
-  Context (SchInSp : sp_incl (SchAS.sp u_s sp_user_s) sp_s).
+
+  Context (sp_mem : string → option fspec).
+  Local Lemma sp_incl_sch : sp_incl (SchAS.sp ∅ sp_empty) (to_sp (SchAS.sp ∅ sp_empty)).
+  Proof.
+    split; ss.
+    rewrite /SchAS.sp; unseal CRIS; ss.
+    prove_nodup.
+  Qed.
 
   Definition Ist : nat → alist key Any.t → alist key Any.t → iProp Σ := λ _ _ _, emp%I.
 
   Local Definition MemA := (MemA.t sp_mem).
-  Local Definition FaaA := (FaaA.t u_s sp_s).
+  Local Definition FaaA := (FaaA.t).
   Local Definition FaaI := (FaaI.t).
   Local Definition IstFull := (IstProd (IstSB FaaA.(HMod.scopes) Ist) IstEq).
   Local Definition MA := (FaaA ★ MemA).
   Local Definition MI := (FaaI ★ MemA).
 
   Lemma faa2_simF : HSim.sim_fun open MA MI IstFull FaaHdr.faa2.
-  Proof using SchInSp.
-    init_simF u_s 0.
+  Proof using.
+    init_simF.
     steps_l. iDestruct "ASM" as "[TID [-> ->]]". hss.
     destruct q2 as [b ofs]. rename q1 into tid.
     steps_l. steps_r.
 
     (* tgt yield *)
-    sch_yield_r.
+    sch_yield_r; eauto.
+    { apply sp_incl_sch. }
     iFrame. clear nths st_src st_tgt NODD NODS. iIntros (nths st_s st_t NODS NODD) "IST TID".
     (* src yield *)
     sch_yield_l.
@@ -47,7 +53,7 @@ Module FaaIA. Section FaaIA.
     (* src give pointsto *)
     force_l. iFrame. steps_l.
     (* tgt yield *)
-    sch_yield_r.
+    sch_yield_r; eauto using sp_incl_sch.
     iFrame. clear nths st_s st_t NODD NODS. iIntros (nths st_s st_t NODS NODD) "IST TID".
     (* src yield *)
     sch_yield_l.
@@ -66,7 +72,7 @@ Module FaaIA. Section FaaIA.
     (* src give pointsto *)
     force_l. iFrame. steps_l.
     (* tgt yield *)
-    sch_yield_r.
+    sch_yield_r; first eauto using sp_incl_sch.
     iFrame. clear nths st_s st_t NODD NODS. iIntros (nths st_s st_t NODS NODD) "IST TID".
     (* tgt terminate *)
     steps_r.
